theories/L6_PCPS/map_util.v
@@ -5,8 +5,8 @@
 From Coq Require Import NArith.BinNat Relations.Relations MSets.MSets
          MSets.MSetRBT Lists.List omega.Omega Sets.Ensembles Relations.Relations
          Classes.Morphisms.
-From CertiCoq.L6 Require Import Ensembles_util set_util functions.
-From compcert.lib Require Import Maps.
+From CertiCoq.L6 Require Import Ensembles_util set_util functions List_util.
+From compcert.lib Require Import Coqlib Maps.
 
 Module M := Maps.PTree. 
 
@@ -75,14 +75,475 @@ Proof.
   eexists (@mset (FromList (map fst (M.elements rho))) _).
   rewrite <- mset_eq, FromList_map_image_FromList.
   split; intros x Hin.
-  - unfold In, key_set in *.
+  - unfold Ensembles.In, key_set in *.
     destruct (M.get x rho) eqn:Hget. 
     eexists (x, a). split; eauto.
     eapply M.elements_correct. eassumption. 
-
     exfalso; eauto.
   - destruct Hin as [[z a] [Hin Hget]]; subst.
-    unfold In, FromList in Hin. eapply M.elements_complete in Hin.
-    simpl. unfold key_set, In. now rewrite Hin.
+    unfold Ensembles.In, FromList in Hin. eapply M.elements_complete in Hin.
+    simpl. unfold key_set, Ensembles.In. now rewrite Hin.
 Qed. 
 
+Definition eq_env_P {A}:  Ensemble M.elt -> M.t A -> M.t A -> Prop :=
+  fun S rho1 rho2 =>
+    forall x, S x -> M.get x rho1 = M.get x rho2.
+
+Lemma eq_env_P_refl: forall {A} S (r:M.t A), eq_env_P S r r.
+Proof.
+  intros; intro; intros. reflexivity.
+Qed.
+
+Lemma eq_env_P_sym: forall {A} S (r:M.t A) r', eq_env_P S r r' -> eq_env_P S r' r.
+Proof.
+  intros; intro. intro. apply H in H0. auto.
+Qed.
+
+Lemma eq_env_P_trans: forall {A} S (r1:M.t A) r2 r3,
+    eq_env_P S r1 r2 -> eq_env_P S r2 r3 -> eq_env_P S r1 r3.
+Proof.
+  intros. intro. intros.
+  specialize (H x H1).
+  specialize (H0 x H1).
+  rewrite H. auto.
+Qed.
+
+Lemma eq_env_P_set_not_in_P_l':
+  forall  {A} (x : M.elt) (v : A)
+          (P : Ensemble M.elt) (rho1 rho2 : M.t A),
+    eq_env_P P  (M.set x v rho1) rho2 ->
+    Disjoint M.elt P (Singleton M.elt x) ->
+    eq_env_P P  rho1 rho2.
+Proof.
+  intros. intro; intros.
+  specialize (H x0 H1).
+  rewrite M.gso in H. auto.
+  intro.
+  inv H0.
+  specialize (H3 x).
+  apply H3; auto.
+Qed.
+
+Fixpoint get_list {A} (xs: list M.elt) (rho: M.t A) : option (list A) :=
+  match xs with
+  | x :: xs' => match M.get x rho, get_list xs' rho with
+               | Some v, Some vs => Some (v::vs)
+               | _, _ => None
+               end
+  | nil => Some nil
+  end.
+
+Fixpoint set_lists {A} (xs: list M.elt) (vs: list A) (rho: M.t A) : option (M.t A) :=
+  match xs, vs with
+  | x::xs', v::vs' => match set_lists xs' vs' rho with
+                     | Some rho' => Some (M.set x v rho')
+                     | None => None
+                     end
+  | nil, nil => Some rho
+  | _, _ => None
+  end.
+
+Definition set_list {A:Type}  (l : list (M.elt * A)) (map: M.t A) : M.t A :=
+  fold_right (fun xv cmap => M.set (fst xv) (snd xv) cmap ) map l.
+
+(** Lemmas about [get_list] *)
+Lemma get_list_In {A} (rho : M.t A) ys x vs :
+  get_list ys rho = Some vs ->
+  List.In x ys ->
+  exists v, M.get x rho = Some v.
+Proof.
+  revert x vs. induction ys; intros x vs Hget H. inv H.
+  inv H; simpl in Hget.
+  - destruct (M.get x rho) eqn:Heq; try discriminate; eauto.
+  - destruct (M.get a rho) eqn:Heq; try discriminate; eauto.
+    destruct (get_list ys rho) eqn:Heq'; try discriminate; eauto.
+Qed.
+
+Lemma In_get_list {A} (xs : list M.elt) (rho : M.t A) :
+  (forall x, List.In x xs -> exists v, M.get x rho = Some v) ->
+  exists vs, get_list xs rho = Some vs.
+Proof.
+  intros H. induction xs.
+  - eexists; simpl; eauto.
+  - edestruct IHxs.
+    + intros x Hin. eapply H. now constructor 2.
+    + edestruct H. now constructor.
+      eexists. simpl. erewrite H1, H0.
+      reflexivity.
+Qed.
+
+Lemma get_list_nth_get {A} (xs : list M.elt) (vs : list A) rho (x : M.elt) N :
+  get_list xs rho = Some vs ->
+  nthN xs N = Some x ->
+  exists v, nthN vs N = Some v /\ M.get x rho = Some v.
+Proof.
+  revert vs N; induction xs; intros vs N Hget Hnth.
+  - inv Hnth.
+  - simpl in Hget.
+    destruct (M.get a rho) eqn:Hget'; try discriminate.
+    destruct (get_list xs rho) eqn:Hget_list'; try discriminate.
+    inv Hget. destruct N.
+    + inv Hnth. eexists; simpl; eauto.
+    + edestruct IHxs as [v' [Hnth1 Hget1]]; eauto.
+Qed.
+
+Lemma get_list_set_neq {A} xs x (v : A) rho :
+  ~ List.In x xs ->
+  get_list xs (M.set x v rho) = get_list xs rho.
+Proof.
+  intros Hin.
+  revert rho. induction xs; intros rho.
+  - reflexivity.
+  - simpl. rewrite M.gso.
+    + rewrite IHxs. reflexivity.
+      intros Hin'. eapply Hin. now constructor 2.
+    + intros Heq; subst. eapply Hin. now constructor.
+Qed.
+
+Lemma get_list_set_lists {A} xs (vs : list A) rho rho' :
+  NoDup xs ->
+  set_lists xs vs rho = Some rho' ->
+  get_list xs rho' = Some vs.
+Proof.
+  revert rho' vs; induction xs; intros rho' vs Hnd Hset.
+  - inv Hset. destruct vs; try discriminate. reflexivity.
+  - inv Hnd. simpl in *.
+    destruct vs; try discriminate.
+    destruct (set_lists xs vs rho) eqn:Hset'; try discriminate. inv Hset.
+    rewrite M.gss. rewrite get_list_set_neq.
+    now erewrite IHxs; eauto. eassumption.
+Qed.
+
+Lemma get_list_set_lists_Disjoint {A} xs xs' (vs : list A) rho rho' :
+  Disjoint _ (FromList xs) (FromList xs') ->
+  set_lists xs vs rho = Some rho' ->
+  get_list xs' rho' = get_list xs' rho.
+Proof with now eauto with Ensembles_DB.
+  revert rho' vs; induction xs; intros rho' vs Hd Hset.
+  - inv Hset. destruct vs; try discriminate. inv H0; reflexivity.
+  - simpl in *.
+    destruct vs; try discriminate.
+    destruct (set_lists xs vs rho) eqn:Hset'; try discriminate. inv Hset.
+    rewrite FromList_cons in Hd.
+    rewrite get_list_set_neq.
+    erewrite IHxs...
+    intros Hc; eapply Hd. constructor; eauto.
+Qed.
+
+Lemma get_list_reset {A} σ x y (v : A) rho l :
+  M.get (σ x) rho = Some v ->
+  ~ y \in (image σ (Setminus _ (FromList l) (Singleton _ x))) ->
+  get_list (map σ l) rho = get_list (map (σ { x ~> y }) l) (M.set y v rho).
+Proof with now eauto with Ensembles_DB.
+  intros Hget Hnin. induction l; eauto.
+  simpl. destruct (peq x a); subst.
+  - rewrite extend_gss, M.gss, Hget.
+    rewrite IHl. reflexivity.
+    intros Hc. eapply Hnin.
+    rewrite FromList_cons.
+    eapply image_monotonic; try eassumption...
+  - rewrite extend_gso; eauto.
+    rewrite M.gso.
+    rewrite IHl. reflexivity.
+    intros Hc. eapply Hnin.
+    rewrite FromList_cons.
+    eapply image_monotonic; try eassumption...
+    intros Hc. eapply Hnin.
+    subst. rewrite FromList_cons. eexists; split; eauto.
+    constructor; eauto.
+    intros Hc; inv Hc. congruence.
+Qed.
+
+Lemma get_list_reset_neq {A} σ x y (v : A) rho l :
+  ~ y \in (image σ (Setminus _ (FromList l) (Singleton _ x))) ->
+  ~ List.In x l ->
+  get_list (map σ l) rho = get_list (map (σ { x ~> y }) l) (M.set y v rho).
+Proof with now eauto with Ensembles_DB.
+  intros  Hnin. induction l; intros Hnin'; eauto.
+  simpl. destruct (peq x a); subst.
+  - exfalso. eapply Hnin'. now constructor.
+  - rewrite extend_gso; eauto.
+    rewrite M.gso.
+    rewrite IHl. reflexivity.
+    intros Hc. eapply Hnin.
+    rewrite FromList_cons.
+    eapply image_monotonic; try eassumption...
+    intros Hc. eapply Hnin'. now constructor 2.
+    intros Hc. subst. eapply Hnin.
+    rewrite FromList_cons. eexists; split; eauto.
+    constructor; eauto.
+    intros Hc; inv Hc. congruence.
+Qed.
+
+Lemma get_eq_get_list_eq {A} (rho rho' : M.t A) xs :
+  (forall z, M.get z rho = M.get z rho') ->
+  get_list xs rho = get_list xs rho'.
+Proof.
+  induction xs; intros H; eauto.
+  simpl; f_equal.
+  rewrite IHxs; eauto.
+  rewrite H. reflexivity.
+Qed.
+
+Lemma get_list_app {A} m l1 l2 (v1 v2 : list A) :
+  get_list l1 m = Some v1 ->
+  get_list l2 m = Some v2 ->
+  get_list (l1 ++ l2) m = Some (v1 ++ v2).
+Proof.
+  revert v1. induction l1; intros v1 Hget1 Hget2; simpl in *.
+  - inv Hget1. eauto.
+  - destruct (M.get a m) eqn:Hgeta; try discriminate.
+    destruct (get_list l1 m) eqn:Hget; try discriminate.
+    inv Hget1. simpl. erewrite IHl1; eauto.
+Qed.
+
+Lemma get_list_length_eq {A} l (vs : list A) rho :
+  get_list l rho = Some vs ->
+  length l = length vs.
+Proof.
+  revert vs; induction l; intros vs Hget.
+  - inv Hget. eauto.
+  - simpl in Hget. destruct (M.get a rho); try discriminate.
+    destruct (get_list l rho); try discriminate.
+    inv Hget. simpl. f_equal; eauto.
+Qed.
+
+Lemma app_get_list {A} l1 l2 (vs : list A) rho :
+  get_list (l1 ++ l2) rho = Some vs ->
+  exists vs1 vs2,
+    get_list l1 rho = Some vs1 /\
+    get_list l2 rho = Some vs2 /\
+    vs = vs1 ++ vs2.
+Proof.
+  revert vs. induction l1; intros vs Hget.
+  - simpl in Hget. repeat eexists; eauto.
+  - simpl in Hget.
+    destruct (M.get a rho) eqn:Hgeta; try discriminate.
+    destruct (get_list (l1 ++ l2) rho) eqn:Hgetl; try discriminate.
+    inv Hget.
+    edestruct IHl1 as [vs1 [vs2 [Hget1 [Hget2 Heq]]]].
+    reflexivity.
+    repeat eexists; eauto. simpl.
+    rewrite Hgeta, Hget1. reflexivity.
+    simpl. congruence.
+Qed.
+
+Lemma get_list_In_val {A} (rho : M.t A) ys v vs :
+  get_list ys rho = Some vs ->
+  List.In v vs ->
+  exists x, List.In x ys /\ M.get x rho = Some v.
+Proof.
+  revert v vs. induction ys; intros x vs Hget H.
+  - inv Hget. now inv H.
+  - simpl in *.
+    destruct (M.get a rho) eqn:Heq; try discriminate; eauto.
+    destruct (get_list ys rho) eqn:Heq'; try discriminate; eauto.
+    inv Hget. inv H; eauto.
+    edestruct IHys as [y [Hin Hget]]; eauto.
+Qed.
+
+
+(** Lemmas about [set_lists]  *)
+
+Lemma set_lists_Forall2_get {A} (P : A -> A -> Prop)
+      xs vs1 vs2 rho1 rho2 rho1' rho2' x :
+  Forall2 P vs1 vs2 ->
+  set_lists xs vs1 rho1 = Some rho1' ->
+  set_lists xs vs2 rho2 = Some rho2' ->
+  List.In x xs ->
+  exists v1 v2,
+    M.get x rho1' = Some v1 /\
+    M.get x rho2' = Some v2 /\ P v1 v2.
+Proof.
+  revert rho1' rho2' vs1 vs2.
+  induction xs; simpl; intros rho1' rho2' vs1 vs2 Hall Hset1 Hset2 Hin.
+  - inv Hin.
+  - destruct (Coqlib.peq a x); subst.
+    + destruct vs1; destruct vs2; try discriminate.
+      destruct (set_lists xs vs1 rho1) eqn:Heq1;
+        destruct (set_lists xs vs2 rho2) eqn:Heq2; try discriminate.
+      inv Hset1; inv Hset2. inv Hall.
+      repeat eexists; try rewrite M.gss; eauto.
+    + destruct vs1; destruct vs2; try discriminate.
+      destruct (set_lists xs vs1 rho1) eqn:Heq1;
+        destruct (set_lists xs vs2 rho2) eqn:Heq2; try discriminate.
+      inv Hset1; inv Hset2. inv Hall. inv Hin; try congruence.
+      edestruct IHxs as [v1 [v2 [Hget1 [Hget2 HP]]]]; eauto.
+      repeat eexists; eauto; rewrite M.gso; eauto.
+Qed.
+
+Lemma get_set_lists_In_xs {A} x xs vs rho rho' :
+  x \in (FromList xs) ->
+  set_lists xs vs rho = Some rho' ->
+  exists v : A, M.get x rho' = Some v.
+Proof.
+  revert rho rho' vs. induction xs; intros rho rho' vs Hin Hset.
+  - rewrite FromList_nil in Hin. exfalso.
+    eapply not_In_Empty_set. eassumption.
+  - rewrite FromList_cons in Hin.
+    destruct vs; try discriminate.
+    simpl in Hset. destruct (set_lists xs vs rho) eqn:Hset_lists; try discriminate.
+    inv Hset. inv Hin.
+    + inv H. eexists. rewrite M.gss. reflexivity.
+    + destruct (Coqlib.peq x a); subst.
+      * eexists. now rewrite M.gss.
+      * edestruct IHxs; eauto.
+        eexists. simpl. rewrite M.gso; eauto.
+Qed.
+
+Lemma set_lists_not_In {A} (xs : list M.elt) (vs : list A)
+      (rho rho' : M.t A) (x : M.elt) :
+  set_lists xs vs rho = Some rho' ->
+  ~ List.In x xs ->
+  M.get x rho = M.get x rho'.
+Proof.
+  revert vs rho'.
+  induction xs; simpl; intros vs rho' Hset Hin.
+  - destruct vs; congruence.
+  - destruct vs; try discriminate.
+    destruct (set_lists xs vs rho) eqn:Heq1; try discriminate. inv Hset.
+    rewrite M.gso; eauto.
+Qed.
+
+Lemma set_lists_length {A} (rho rho' rho1 : M.t A)
+      (xs : list M.elt) (vs1 vs2 : list A) :
+  length vs1 = length vs2 ->
+  set_lists xs vs1 rho = Some rho1 ->
+  exists rho2, set_lists xs vs2 rho' = Some rho2.
+Proof.
+  revert vs1 vs2 rho1.
+  induction xs as [| x xs IHxs ]; intros vs1 vs2 rho1 Hlen Hset.
+  - inv Hset. destruct vs1; try discriminate. inv H0.
+    destruct vs2; try discriminate. eexists; simpl; eauto.
+  - destruct vs1; try discriminate. destruct vs2; try discriminate.
+    inv Hlen. simpl in Hset.
+    destruct (set_lists xs vs1 rho) eqn:Heq2; try discriminate.
+    edestruct (IHxs _ _ _ H0 Heq2) as  [vs2' Hset2].
+    eexists. simpl; rewrite Hset2; eauto.
+Qed.
+
+Lemma set_permut {A} rho x y (v1 v2 : A) z :
+  x <> y ->
+  M.get z (M.set x v1 (M.set y v2 rho)) =
+  M.get z (M.set y v2 (M.set x v1 rho)).
+Proof.
+  intros Hnin. destruct (peq z x); subst.
+  - rewrite M.gss, M.gso, M.gss; eauto.
+  - rewrite (@M.gso _ z x); eauto.
+    destruct (peq z y); subst.
+    + rewrite !M.gss; eauto.
+    + rewrite !M.gso; eauto.
+Qed.
+
+Lemma set_set_lists_permut {A} rho rho' y ys (v : A) vs :
+  set_lists ys vs rho = Some rho' ->
+  ~ List.In y ys ->
+  exists rho'',
+    set_lists ys vs (M.set y v rho) = Some rho'' /\
+    (forall z, M.get z (M.set y v rho') = M.get z rho'').
+Proof.
+  revert vs rho'.
+  induction ys; intros vs rho' Hset Hin;
+  destruct vs; try discriminate.
+  - inv Hset. eexists; split; simpl; eauto.
+  - simpl in Hset.
+    destruct (set_lists ys vs rho) eqn:Heq; try discriminate.
+    inv Hset. edestruct IHys as [rho'' [Hset Hget]]; eauto.
+    intros Hc; eapply Hin; now constructor 2.
+    eexists; split.
+    simpl. rewrite Hset. reflexivity.
+    intros z. rewrite set_permut.
+    destruct (peq z a); subst.
+    + rewrite !M.gss; eauto.
+    + rewrite !(@M.gso _ z a); eauto.
+    + intros Hc. eapply Hin.
+      constructor; eauto.
+Qed.
+
+Lemma set_lists_length3 {A} (rho : M.t A) xs vs :
+  length xs = length vs ->
+  exists rho', set_lists xs vs rho = Some rho'.
+Proof.
+  revert vs; induction xs; intros vs Hlen; destruct vs; try discriminate.
+  - eexists; simpl; eauto.
+  - inv Hlen.
+    edestruct IHxs as [rho' Hset]. eassumption.
+    eexists. simpl. rewrite Hset. reflexivity.
+Qed.
+
+Lemma set_lists_app {A} xs1 xs2 (vs1 vs2 : list A) rho rho' :
+  set_lists (xs1 ++ xs2) (vs1 ++ vs2) rho = Some rho' ->
+  length xs1 = length vs1 ->
+  exists rho'',
+    set_lists xs2 vs2 rho = Some rho'' /\
+    set_lists xs1 vs1 rho'' = Some rho'.
+Proof.
+  revert vs1 rho'. induction xs1; intros vs1 rho' Hset Hlen.
+  - destruct vs1; try discriminate.
+    eexists; split; eauto.
+  - destruct vs1; try discriminate.
+    inv Hlen. simpl in Hset.
+    destruct (set_lists (xs1 ++ xs2) (vs1 ++ vs2) rho) eqn:Heq; try discriminate.
+    inv Hset. edestruct IHxs1 as [rho'' [Hset1 Hset2]].
+    eassumption. eassumption.
+    eexists. split. eassumption. simpl; rewrite Hset2; reflexivity.
+Qed.
+
+
+Lemma set_lists_length_eq {A} rho rho' xs (vs : list A) :
+  set_lists xs vs rho = Some rho' ->
+  length xs = length vs.
+Proof.
+  revert rho' vs; induction xs; intros rho' vs Hset.
+  - destruct vs; try discriminate. reflexivity.
+  - destruct vs; try discriminate.
+    simpl in Hset.
+    destruct (set_lists xs vs rho) eqn:Heq; try discriminate.
+    simpl. f_equal. inv Hset. eauto.
+Qed.
+
+Lemma get_list_reset_lst {A} σ xs ys (vs : list A) rho rho' l  :
+  set_lists ys vs rho = Some rho' ->
+  get_list (map σ xs) rho = Some vs ->
+  Disjoint _ (image σ (FromList l)) (FromList ys) ->
+  length xs = length ys ->
+  NoDup xs -> NoDup ys ->
+  get_list (map σ l) rho = get_list (map (σ <{ xs ~> ys }>) l) rho'.
+Proof with now eauto with Ensembles_DB.
+  revert σ ys vs rho' rho. induction xs as [| x xs IHxs ];
+    intros σ ys vs rho' rho Hset Hget HD Hlen Hnd1 Hnd2.
+  - destruct ys; try discriminate.
+    inv Hget. inv Hset. reflexivity.
+  - destruct ys; try discriminate. simpl in *.
+    inv Hlen. destruct vs as [| v vs]; try discriminate.
+    destruct (set_lists ys vs rho) eqn:Hset'; try discriminate.
+    destruct (M.get (σ x) rho) eqn:Hget'; try discriminate.
+    destruct (get_list (map σ xs) rho) eqn:Hgetl; try discriminate.
+    inv Hget. inv Hset. inv Hnd1. inv Hnd2. rewrite !FromList_cons in HD.
+    assert (H : get_list (map ((σ <{ xs ~> ys }>) {x ~> e}) l) (M.set e v t) =
+                get_list (map ((σ <{ xs ~> ys }>)) l) t).
+    { destruct (in_dec peq x l).
+      - rewrite <- get_list_reset; try reflexivity.
+        rewrite extend_lst_gso; eauto.
+        erewrite <- set_lists_not_In. eassumption. eassumption.
+        intros Hc. eapply HD. constructor; eauto.
+        eexists; split; eauto.
+        intros Hc.
+        apply image_extend_lst_Included in Hc; eauto.
+        inv Hc; eauto. eapply HD. constructor; eauto.
+        eapply image_monotonic; [| eassumption ]...
+      - rewrite map_extend_not_In; eauto.
+        erewrite get_list_set_neq. reflexivity.
+        intros Hc. eapply in_map_iff in Hc.
+        destruct Hc as [x' [Heq Hin]].
+        destruct (in_dec peq x' xs).
+        + edestruct (extend_lst_gss σ) as [y' [Hin' Heq']]; eauto.
+          rewrite Heq in Hin'. subst.
+          subst. eauto.
+        + rewrite extend_lst_gso in Heq; eauto.
+          eapply HD. constructor; eauto.
+          eexists; eauto. }
+    rewrite H.
+    erewrite <- IHxs; eauto.
+    now eauto with Ensembles_DB.
+Qed.
