theories/L6_PCPS/alpha_conv.v
@@ -785,25 +785,20 @@ Section Alpha_conv_correct.
         eexists. rewrite M.gso; eauto. 
   Qed.
   
-  Lemma preord_env_P_inj_set_alt (S : Ensemble var) (rho1 rho2 : env) 
+  Lemma preord_env_P_inj_set_l (S : Ensemble var) (rho1 rho2 : env) 
         (k : nat) f (x y : var) (v1 v2 : val) : 
     preord_env_P_inj (S \\ [set x]) k f rho1 rho2 ->
     preord_val cenv PG k v1 v2 ->
-    ~ In _ (image f (S \\ [set x])) y ->
-    preord_env_P_inj S k (f {x ~> y}) (M.set x v1 rho1) (M.set y v2 rho2).
+    M.get y rho2 = Some v2 ->
+    preord_env_P_inj S k (f {x ~> y}) (M.set x v1 rho1) rho2.
   Proof.
     intros Henv Hv Hnin z HP. unfold extend. 
     destruct (peq z x) as [| Hneq].
     - subst. intros z Hget.
-      rewrite M.gss in Hget. inv Hget. eexists. rewrite M.gss; eauto.
+      rewrite M.gss in Hget. inv Hget. eexists. split; eauto.
     - intros z' Hget. rewrite M.gso in Hget; eauto.
-      destruct (peq (f z) y).
-      + exfalso. eapply Hnin. eexists; eauto.
-        split; eauto. constructor; eauto.
-        intros Hc; inv Hc; congruence.
-      + edestruct (Henv z); eauto.
-        constructor; eauto. intros Hc. inv Hc. congruence. 
-        eexists. rewrite M.gso; eauto. 
+      eapply Henv. constructor; eauto. intros Hc; inv Hc; eauto.
+      eassumption.  
   Qed.
 
   Lemma preord_env_P_inj_antimon (S1 S2 : var -> Prop) (k : nat) (rho1 rho2 : env) f :
